Coherence/Restrict.v
@@ -1,4 +1,4 @@
-Require Import CSet Util Get Drop Var Map Infra.Relations AllInRel OUnion MoreList.
+Require Import CSet Util Get Drop Var Map OptionR AllInRel OUnion MoreList.
 
 Set Implicit Arguments.
 
