IL/Annotation.v
@@ -1,6 +1,6 @@
-Require Import List.
-Require Import Util Relations Get Drop Var Val Exp Env Map CSet AutoIndTac MoreList IL DecSolve.
-Require Import PartialOrder.
+Require Import List AllInRel.
+Require Import Util Get Drop Var Val Exp Env Map CSet AutoIndTac MoreList IL DecSolve.
+Require Import PartialOrder Terminating .
 
 Set Implicit Arguments.
 
@@ -310,4 +310,87 @@ Lemma getAnn_mapAnn_map (A B:Type) (f:A->B) L
 Proof.
   rewrite map_map. setoid_rewrite getAnn_mapAnn.
   rewrite <- map_map. reflexivity.
+Qed.
+
+Lemma terminating_ann Dom `{PO:PartialOrder Dom}
+  : Terminating Dom poLt
+    -> Terminating (ann Dom) poLt.
+Proof.
+  intros Trm a.
+  econstructor. intros ? [A _].
+  induction A.
+  - specialize (Trm b).
+    general induction Trm.
+    econstructor. intros ? [A B].
+    inv A.
+    eapply H0; eauto. split; eauto.
+    intro. eapply B. econstructor. eauto.
+  - pose proof (Trm b) as FST. clear A H.
+    rename IHA into SND.
+    assert (poLe bn bn) by reflexivity.
+    revert H. generalize bn at 2 3.
+    induction FST as [? ? FST].
+    assert (poLe x x) by reflexivity.
+    revert H0. generalize x at 2 3.
+    induction SND as [? ? SND].
+    intros.
+    econstructor; intros ? [A B].
+    inv A.
+    decide (poEq bn bn0).
+    + decide (poEq x1 b).
+      exfalso; eapply B; econstructor; eauto.
+      eapply FST; eauto.
+    + eapply (SND bn0); eauto.
+  - clear H A1 A2 ans ant a.
+    assert (poLe bns bns) by reflexivity.
+    revert H. generalize bns at 2 3.
+    assert (poLe bnt bnt) by reflexivity.
+    revert H. generalize bnt at 2 3.
+    assert (poLe b b) by reflexivity.
+    revert H. generalize b at 2 3.
+    specialize (Trm b).
+    induction Trm.
+    induction IHA1.
+    induction IHA2.
+    intros.
+    econstructor; intros ? [A B].
+    inv A.
+    decide (poEq b b0).
+    + decide (poEq bns bns0).
+      * decide (poEq bnt bnt0).
+        exfalso; apply B; econstructor; eauto.
+        eapply (H4 bnt0); eauto.
+      * eapply (H2 bns0); eauto.
+    + eapply (H0 b0); eauto.
+  - clear H A.
+    pose proof (Trm b) as FST.
+    rename IHA into SND.
+    assert (TRD:terminates poLt bns). {
+      eapply terminates_list_get.
+      intros. symmetry in H0; edestruct get_length_eq; eauto.
+    }
+    clear H0 H1 H2.
+    assert (poLe bns bns) by reflexivity.
+    revert H. generalize bns at 2 3.
+    assert (poLe bnt bnt) by reflexivity.
+    revert H. generalize bnt at 2 3.
+    assert (poLe b b) by reflexivity.
+    revert H. generalize b at 2 3.
+    induction FST.
+    induction SND.
+    induction TRD.
+    intros.
+    econstructor; intros ? [A B].
+    inv A.
+    decide (poEq b b0).
+    + decide (poEq bns bns0).
+      * decide (poEq bnt bnt0).
+        exfalso; apply B; eauto. econstructor; eauto.
+        intros. eapply PIR2_nth in p0; eauto.
+        dcr. get_functional. eauto.
+        eapply (H2 bnt0); eauto.
+      * eapply PIR2_get in H14; eauto.
+        eapply (H4 bns0); eauto.
+    + eapply PIR2_get in H14; eauto.
+      eapply (H0 b0); eauto.
 Qed.
