IL/IL.v
@@ -1,5 +1,5 @@
 Require Import List.
-Require Export Util Relations Get Drop Var Val Exp Env Map CSet AutoIndTac MoreList OptionMap.
+Require Export Util Get Drop Var Val Exp Env Map CSet AutoIndTac MoreList OptionMap.
 Require Export Events SizeInduction SmallStepRelations StateType.
 Require Import SetOperations.
 
