IL/Rename.v
@@ -1,5 +1,5 @@
 Require Import List.
-Require Export Util Relations Get Drop Var Val Exp Env Map CSet AutoIndTac MoreList OptionMap Events.
+Require Export Util Get Drop Var Val Exp Env Map CSet AutoIndTac MoreList OptionMap Events.
 Require Import SetOperations IL.
 
 Set Implicit Arguments.
